one more level of translation: invertible binds

dev2015/dot-stp-single3.v
@@ -7,17 +7,17 @@ Require Export Arith.Le.
 (* 
 subtyping: 
   - looking at single-environment case again.
+  - new pushback proof structure: transitivity axiom only 
+    needed in contravariant positions
+  - realizable type: precise expansion, and upper bounds 
+    are also realizable
 
-  - WIP: trying to figure out pushback story for binds.
-
-    this version explores an stp metric based on n levels
-    of trans-freedom, with n incremented when going into
-    bounds.
-
-    the trans pushback statement holds for n levels if
-    there is realizability evidence for n levels of bounds
-    and if the environment is concrete at level 0.
-
+ TODO/QUESTIONs:
+  - bind2/bind1 rules?
+  - intersection/union types?
+  - restrictions: recursive members?
+  - if lower bound is bottom, must upper bound still be realizable?
+    --> cannot be part of nontrivial T1 < x.A < T2 chain
 *)
 
 
@@ -61,6 +61,10 @@ Fixpoint dc_type_and (dcs: list(nat*dc)) :=
     | (n, dfun T1 T2 _ _)::dcs =>
       TAnd (TFun (length dcs) T1 T2)  (dc_type_and dcs)
   end.
+
+
+Definition TObj p dcs := TAnd (TMem p p) (dc_type_and dcs).
+Definition TArrow p x y := TAnd (TMem p p) (TAnd (TFun 0 x y) TNoF).
 
 
 Inductive vl : Type :=
@@ -144,6 +148,11 @@ Fixpoint open_rec (k: nat) (u: id) (T: ty) { struct T }: ty :=
 
 Definition open u T := open_rec 0 u T.
 
+(* sanity check *)
+Example open_ex1: open 9 (TBind (TAnd (TMem TBot TTop) (TFun 0 (TSelB 1) (TSelB 0)))) =
+                      (TBind (TAnd (TMem TBot TTop) (TFun 0 (TSel  9) (TSelB 0)))).
+Proof. compute. eauto. Qed.
+
 
 Lemma closed_no_open: forall T x j,
   closed_rec j T ->
@@ -178,95 +187,488 @@ Hint Unfold closed.
 (* Static properties: type assignment, subtyping, ... *)
 (* ############################################################ *)
 
+(* TODO: wf is not up to date *)
+
+(* static type expansion.
+   needs to imply dynamic subtyping / value typing. *)
+Inductive tresolve: id -> ty -> ty -> Prop :=
+  | tr_self: forall x T,
+             tresolve x T T
+  | tr_and1: forall x T1 T2 T,
+             tresolve x T1 T ->
+             tresolve x (TAnd T1 T2) T
+  | tr_and2: forall x T1 T2 T,
+             tresolve x T2 T ->
+             tresolve x (TAnd T1 T2) T
+  | tr_unpack: forall x T2 T3 T,
+             open x T2 = T3 ->
+             tresolve x T3 T ->
+             tresolve x (TBind T2) T
+.
+
+Tactic Notation "tresolve_cases" tactic(first) ident(c) :=
+  first;
+  [ Case_aux c "Self" |
+    Case_aux c "And1" |
+    Case_aux c "And2" |
+    Case_aux c "Bind" ].
+
+
+(* static type well-formedness.
+   needs to imply dynamic subtyping. *)
+Inductive wf_type : tenv -> ty -> Prop :=
+| wf_top: forall env,
+    wf_type env TNoF
+| wf_bool: forall env,
+    wf_type env TBool
+| wf_and: forall env T1 T2,
+             wf_type env T1 ->
+             wf_type env T2 ->
+             wf_type env (TAnd T1 T2)
+| wf_mem: forall env TL TU,
+             wf_type env TL ->
+             wf_type env TU ->
+             wf_type env (TMem TL TU)
+| wf_fun: forall env f T1 T2,
+             wf_type env T1 ->
+             wf_type env T2 ->
+             wf_type env (TFun f T1 T2)
+                     
+| wf_sel: forall envz x TE TL TU,
+            index x envz = Some (TE) ->
+            tresolve x TE (TMem TL TU) ->
+            wf_type envz (TSel x)
+
+| wf_selb: forall envz x, (* note: disregarding bind-scope *)
+             wf_type envz (TSelB x)
+| wf_bind: forall envz T,
+             wf_type envz T ->
+             wf_type envz (TBind T)
+
+.
+
+Tactic Notation "wf_cases" tactic(first) ident(c) :=
+  first;
+  [ Case_aux c "Top" |
+    Case_aux c "Bool" |
+    Case_aux c "And" |
+    Case_aux c "MemA" |
+    Case_aux c "Mem" |
+    Case_aux c "Fun" |
+    Case_aux c "Sel" |
+    Case_aux x "SelB" |
+    Case_aux c "Bind" ].
+
+
+
 (* this is the version we can narrow *)
 
-Fixpoint plus (a: list nat) (b: list nat) :=
-  match a,b with
-    | x::xs, y::ys => (x+y)::(plus xs ys)
-    | nil, ys => ys
-    | xs, nil => xs
-  end.
+Inductive stp : bool -> tenv -> ty -> ty -> nat -> Prop := 
 
-Fixpoint less (a: list nat) (b: list nat): Prop :=
-  match a,b with
-    | x::xs, y::ys => x < y \/ (x = y /\ less xs ys)
-    | xs, ys => xs = nil
-end.
+| stp_bot: forall G1 T n1,
+    stp true G1 TBot T n1
 
-Inductive itp: nat -> ty -> Prop :=
-| itp_refl: forall T,
-    itp 0 T
-| itp_mem: forall T n,
-    itp n T ->
-    itp (S n) (TMem T T).
-
-
-Inductive stp : nat -> tenv -> ty -> ty -> nat -> Prop := 
-
-| stp_bot: forall G1 T n1 d1,
-    stp (S d1) G1 TBot T (S n1)
+| stp_top: forall G1 T n1,
+    stp true G1 T TTop n1
              
-| stp_top: forall G1 T n1 d1,
-    stp (S d1) G1 T TTop (S n1)
-             
-| stp_bool: forall G1 n1 d1,
-    stp (S d1) G1 TBool TBool (S n1)
+| stp_bool: forall G1 n1,
+    stp true G1 TBool TBool n1
 
-| stp_fun: forall m G1 T11 T12 T21 T22 n1 n2 d3,
-    stp 0 G1 T21 T11 n1 ->
-    stp 0 G1 T12 T22 n2 ->
-    stp (S d3) G1 (TFun m T11 T12) (TFun m T21 T22) (S (n1+n2))
+| stp_fun: forall m G1 T11 T12 T21 T22 n1 n2,
+    stp false G1 T21 T11 n1 ->
+    stp true G1 T12 T22 n2 ->
+    stp true G1 (TFun m T11 T12) (TFun m T21 T22) (S (n1+n2))
 
-| stp_mem: forall G1 T11 T12 T21 T22 n1 n2 d2,
-    stp 0 G1 T21 T11 n1 ->
-    stp d2 G1 T12 T22 n2 ->
-    stp (S d2) G1 (TMem T11 T12) (TMem T21 T22) (S (n1+n2))
-
-(*
-| stp_sel2: forall x T1 TX G1 n1 d1,
-    index x G1 = Some (TMem TX) ->
-    stp d1 G1 T1 TX n1 ->
-    stp d1 G1 T1 (TSel x) (S n1)
-| stp_sel1: forall x T2 TX G1 n1 d1,
-    index x G1 = Some (TMem TX) ->
-    stp d1 G1 TX T2 n1 ->
-    stp d1 G1 (TSel x) T2 (S n1)
-*)
+| stp_mem: forall G1 T11 T12 T21 T22 n1 n2 n3,
+    stp false G1 T21 T11 n1 ->
+    stp true G1 T11 T12 n2 -> (* NOT SO EASY TO ADD: build_mem! *)
+    stp true G1 T12 T22 n3 ->
+    stp true G1 (TMem T11 T12) (TMem T21 T22) (S (n1+n2+n3))
         
-| stp_sel2: forall x T1 TX G1 n1 d1,
+| stp_sel2: forall x T1 TX G1 n1,
     index x G1 = Some TX ->
-    itp d1 TX ->          
-    stp d1 G1 TX (TMem T1 TTop) n1 ->
-    stp d1 G1 T1 (TSel x) (S n1)
-| stp_sel1: forall x T2 TX G1 n1 d1,
+    stp false G1 TX (TMem T1 TTop) n1 ->
+    stp true G1 T1 (TSel x) (S n1)
+| stp_sel1: forall x T2 TX G1 n1,
     index x G1 = Some TX ->
-    itp d1 TX ->          
-    stp d1 G1 TX (TMem TBot T2) n1 ->
-    stp d1 G1 (TSel x) T2 (S n1)
-
-
-| stp_selx: forall x G1 n1 d1,
-    stp (S d1) G1 (TSel x) (TSel x) (S n1)
+    stp false G1 TX (TMem TBot T2) n1 ->
+    stp true G1 (TSel x) T2 (S n1)
+| stp_selx: forall x G1 n1,
+    stp true G1 (TSel x) (TSel x) (S n1)
                   
-| stp_bindx: forall G1 T1 T2 TA1 TA2 n1 d1,
-    stp (S d1) ((length G1,T1)::G1) T1 T2 n1 ->
+(* TODO!
+| stp_bind2: forall f G1 T1 T2 TA2 n1,
+    stp true ((f,T1)::G1) T1 T2 n1 ->
+    open (length G1) TA2 = T2 ->                
+    stp true G1 T1 (TBind TA2) (S n1)
+| stp_bind1: forall f G1 T1 T2 TA1 n1,
+    stp true ((f,T1)::G1) T1 T2 n1 ->
+    open (length G1) TA1 = T1 ->                
+    stp true G1 (TBind TA1) T2 (S n1)
+... or at least...
+*)
+| stp_bindx: forall G1 T1 T2 TA1 TA2 n1,
+    stp false ((length G1,T1)::G1) T1 T2 n1 ->
     open (length G1) TA1 = T1 ->                
     open (length G1) TA2 = T2 ->
-    stp (S d1) G1 (TBind TA1) (TBind TA2) (S n1)
+    stp true G1 (TBind TA1) (TBind TA2) (S n1)
 
-| stp_wrapf: forall G1 T1 T2 n1 d,
-    stp d G1 T1 T2 n1 ->
-    stp 0 G1 T1 T2 (S n1)
+| stp_transf: forall G1 T1 T2 T3 n1 n2,
+    stp true G1 T1 T2 n1 ->
+    stp false G1 T2 T3 n2 ->           
+    stp false G1 T1 T3 (S (n1+n2))
 
-| stp_transf: forall G1 T1 T2 T3 n1 n2 d,
-    stp d G1 T1 T2 n1 ->
-    stp 0 G1 T2 T3 n2 ->
-    stp 0 G1 T1 T3 (S (n1+n2)) 
+| stp_wrapf: forall G1 T1 T2 n1,
+    stp true G1 T1 T2 n1 ->
+    stp false G1 T1 T2 (S n1)       
 .
+
+
+(* implementable types *)
+Inductive itp: tenv -> ty -> nat -> Prop :=
+
+| itp_top: forall G1 n1,
+    itp G1 TTop n1
+| itp_bool: forall G1 n1,
+    itp G1 TBool n1
+(* TODO: we should have another mem case,
+   if lower bound is bot, upper bound need
+   not be realizable (?) *)
+| itp_mem: forall G1 TL TU n1 n2,
+(*    stp true G1 TL TU n1 -> (* may or may not be needed *) *)
+    itp G1 TU n2 -> 
+    itp G1 (TMem TL TU) (S (n1+n2))
+| itp_bind: forall G1 T1 TA1 n1,
+    itp ((length G1,T1)::G1) T1 n1 ->  (* TAKING THE OTHER ONE *)
+    open (length G1) TA1 = T1 ->
+    itp G1 (TBind TA1) (S n1)
+| itp_sel: forall G1 TX x n1,
+    index x G1 = Some TX ->
+    itp G1 TX n1 -> (* could / should we rely on env_itp to provide this? *)
+    itp G1 (TSel x) (S n1)
+.
+
+
+
+
+(* this is the version we can trans *)
+
+Inductive stp2 : bool -> tenv -> ty -> ty -> nat -> Prop := 
+
+| stp2_bot: forall G1 T n1,
+    stp2 true G1 TBot T n1
+
+| stp2_top: forall G1 T n1,
+    stp2 true G1 T TTop n1
+             
+| stp2_bool: forall G1 n1,
+    stp2 true G1 TBool TBool n1
+
+| stp2_fun: forall m G1 T11 T12 T21 T22 n1 n2,
+    stp2 false G1 T21 T11 n1 ->
+    stp2 true G1 T12 T22 n2 ->
+    stp2 true G1 (TFun m T11 T12) (TFun m T21 T22) (S (n1+n2))
+
+| stp2_mem: forall G1 T11 T12 T21 T22 n1 n2 n3,
+    stp2 false G1 T21 T11 n1 ->
+    stp2 true G1 T11 T12 n2 -> (* NOT SO EASY TO ADD: build_mem! *)
+    stp2 true G1 T12 T22 n3 ->
+    stp2 true G1 (TMem T11 T12) (TMem T21 T22) (S (n1+n2+n3))
+        
+| stp2_sel2: forall x T1 TX G1 n1 n2,
+    index x G1 = Some TX ->
+    itp G1 TX n2 -> 
+    stp2 true G1 TX (TMem T1 TTop) n1 ->
+    stp2 true G1 T1 (TSel x) (S (n1+n2))
+| stp2_sel1: forall x T2 TX G1 n1 n2,
+    index x G1 = Some TX ->
+    itp G1 TX n2 ->
+    stp2 true G1 TX (TMem TBot T2) n1 ->
+    stp2 true G1 (TSel x) T2 (S (n1+n2))
+| stp2_selx: forall x G1 n1,
+    stp2 true G1 (TSel x) (TSel x) (S n1)
+                  
+(* TODO!
+| stp_bind2: forall f G1 T1 T2 TA2 n1,
+    stp true ((f,T1)::G1) T1 T2 n1 ->
+    open (length G1) TA2 = T2 ->                
+    stp true G1 T1 (TBind TA2) (S n1)
+| stp_bind1: forall f G1 T1 T2 TA1 n1,
+    stp true ((f,T1)::G1) T1 T2 n1 ->
+    open (length G1) TA1 = T1 ->                
+    stp true G1 (TBind TA1) T2 (S n1)
+... or at least...
+*)
+| stp2_bindx: forall G1 T1 T2 TA1 TA2 n1,
+    stp false ((length G1,T1)::G1) T1 T2 n1 ->  (* TAKING THE OTHER ONE *)
+    open (length G1) TA1 = T1 ->                
+    open (length G1) TA2 = T2 ->
+    (* no itp here, needs to come from env_itp if extracting things *)
+    (* itp ((length G1,T1)::G1) T1 n2 -> *)
+    stp2 true G1 (TBind TA1) (TBind TA2) (S n1)
+
+| stp2_transf: forall G1 T1 T2 T3 n1 n2,
+    stp2 true G1 T1 T2 n1 ->
+    stp2 false G1 T2 T3 n2 ->           
+    stp2 false G1 T1 T3 (S (n1+n2))
+
+| stp2_wrapf: forall G1 T1 T2 n1,
+    stp2 true G1 T1 T2 n1 ->
+    stp2 false G1 T1 T2 (S n1)       
+.
+
+
+Definition itp2 a b c := itp a b c.
+
+
+(* this is the version that has invertible bindx *)
+
+Inductive stp3 : bool -> tenv -> ty -> ty -> nat -> Prop := 
+
+| stp3_bot: forall G1 T n1,
+    stp3 true G1 TBot T n1
+
+| stp3_top: forall G1 T n1,
+    stp3 true G1 T TTop n1
+             
+| stp3_bool: forall G1 n1,
+    stp3 true G1 TBool TBool n1
+
+| stp3_fun: forall m G1 T11 T12 T21 T22 n1 n2,
+    stp2 false G1 T21 T11 n1 ->
+    stp2 true G1 T12 T22 n2 ->
+    stp3 true G1 (TFun m T11 T12) (TFun m T21 T22) (S (n1+n2))
+
+| stp3_mem: forall G1 T11 T12 T21 T22 n1 n2,
+    stp2 false G1 T21 T11 n1 ->
+    stp3 true G1 T12 T22 n2 ->
+    stp3 true G1 (TMem T11 T12) (TMem T21 T22) (S (n1+n2))
+        
+| stp3_sel2: forall x T1 TX G1 n1 n2,
+    index x G1 = Some TX ->
+    itp G1 TX n2 -> 
+    stp3 true G1 TX (TMem T1 TTop) n1 ->
+    stp3 true G1 T1 (TSel x) (S (n1+n2))
+| stp3_sel1: forall x T2 TX G1 n1 n2,
+    index x G1 = Some TX ->
+    itp G1 TX n2 ->
+    stp3 true G1 TX (TMem TBot T2) n1 ->
+    stp3 true G1 (TSel x) T2 (S (n1+n2))
+| stp3_selx: forall x G1 n1,
+    stp3 true G1 (TSel x) (TSel x) (S n1)
+                  
+| stp3_bindx: forall G1 T1 T2 TA1 TA2 n1 n2,
+    stp3 true ((length G1,T1)::G1) T1 T2 n1 -> (* CAN INVERT *)
+    open (length G1) TA1 = T1 ->                
+    open (length G1) TA2 = T2 ->
+    itp ((length G1,T1)::G1) T1 n2 -> 
+    stp3 true G1 (TBind TA1) (TBind TA2) (S (n1+n2))
+
+| stp3_transf: forall G1 T1 T2 T3 n1 n2,
+    stp3 true G1 T1 T2 n1 ->
+    stp3 false G1 T2 T3 n2 ->           
+    stp3 false G1 T1 T3 (S (n1+n2))
+
+| stp3_wrapf: forall G1 T1 T2 n1,
+    stp3 true G1 T1 T2 n1 ->
+    stp3 false G1 T1 T2 (S n1)       
+.
+
+
+Definition itp3 a b c := itp a b c.
+
+
+
+
+(*
+XXXX ---- XXXX
+
+intersection case for narrowing:
+
+(1) bad bounds
+
+x:Bot..Top, y:Hi..Hi
+x.A /\ y.B,     
+
+narrow x to Lo..Lo
+
+now x.A /\ y.B has bad bounds Hi..Lo
+
+but this object can't exist, it cannot be in context, so all is good !!!
+
+however, the original type can be in context, and this is the trouble case.
+(because we need to show it remains implementable in narrowing).
+
+similarly, the original type can be the body of a self type.
+
+x={A:Bot..{B:Bot..Top}}
+{z => x.A & {B:Hi..Hi }}
+
+narrow x to {A:Bot..{B:Lo..Lo}} 
+
+the context is still implementable,
+but z's body is no longer implementable.
+
+but how can the narrowing happen? x must be bound by a self type...
+
+maybe this will constrain things?
+
+
+
+(2) expansion can be lost already, without looking at bounds
+
+*)
+
+
+
+
+
+
+(*
+
+what about intersection types:
+
+STP
+
+  T <: T1,  T <: T2
+  -----------------
+  T <: T1 /\ T2
+
+
+  T1 <: T,  T2 wfe
+  ----------------
+  T1 /\ T2 <: T
+
+
+  T1 wfe,  T2 <: T 
+  ----------------
+  T1 /\ T2 <: T
+
+
+EXP
+
+  T1 <x {A: L1..U1},  T2 <x {A: L2..U2}
+  ------------------------------------
+  T1 /\ T2 <x {A: L1 \/ L2 .. U1 /\ U2 }
+
+
+  T1 <x {A: L1..U1},  A not in dom(T2)
+  ------------------------------------
+  T1 /\ T2 <x {A: L1..U1}
+
+
+  A not in dom(T1),  T2 <x {A: L2..U2}
+  ------------------------------------
+  T1 /\ T2 <x {A: L2..U2}
+
+
+Problem case (bad bounds):
+
+  (Int..Int) /\ (String..String)
+
+Expansion:
+
+  (Int \/ String) .. (Int /\ String) <--- not <:
+
+
+CONSTRAINTS:
+  - need good bounds (L < U) for stpd_trans_cross
+  - not part of regular stp. needs to come from env
+  - but need to be able to do induction on it
+
+HYPOTHESIS:
+  - put itp in stp_sel1,sel2 evidence: this mirrors 
+    env_itp, but enables induction
+  - narrow uses env_itp to get new itp (output size 
+    doesn't matter)
+
+
+
+Need itp_exp (example):
+
+  itp (L1..U1) /\ (L2..U2)
+  (L1..U1) /\ (L2..U2) <: L..U  [n+1]
+--->
+  (L1..U1) /\ (L2..U2)  <x  (L1 \/ L2 .. U1 /\ U2)
+  (L1 \/ L2  <:  U1 /\ U2)   [n]
+  
+  (L1 \/ L2 .. U1 /\ U2)  <:  L..U
+  itp U1 /\ U2
+*)
+
+
+
+
+
+
+
+
+Tactic Notation "stp_cases" tactic(first) ident(c) :=
+  first;
+  [ 
+    Case_aux c "Bot < ?" |
+    Case_aux c "? < Top" |
+    Case_aux c "Bool < Bool" |
+    Case_aux c "Fun < Fun" |
+    Case_aux c "Mem < Mem" |
+    Case_aux c "? < Sel" |
+    Case_aux c "Sel < ?" |
+    Case_aux c "Sel < Sel" |
+    Case_aux c "Bind < Bind" |
+    Case_aux c "Trans" |
+    Case_aux c "Wrap"
+  ].
+
 
 Hint Resolve ex_intro.
 
 Hint Constructors stp.
+Hint Constructors itp.
+Hint Constructors stp2.
+Hint Constructors stp3.
+
+
+(* ############################################################ *)
+(* Examples *)
+(* ############################################################ *)
+
+
+(*
+THIS IS NOW FALSE: lhs must expand.
+
+Example ex1: exists n, stp true nil (TBind TBot) (TBind TTop) n.
+Proof.
+ eexists. eapply stp_bindx. eapply stp_bot. eauto. (* false - bot doesn't exp! *).
+Grab Existential Variables. apply 0.
+Qed.
+ *)
+
+Example ex2: exists n, stp true nil
+   (TBind (TMem TBool TBool))
+   (TBind (TMem TBot TTop)) n.
+Proof.
+  eexists. eapply stp_bindx. eapply stp_wrapf. eapply stp_mem.  eapply stp_wrapf. eapply stp_bot.
+  eapply stp_bool.
+  eapply stp_top. compute. eauto. compute. eauto. 
+Grab Existential Variables. apply 0. apply 0. apply 0. 
+Qed.
+
+Example ex3: exists n, stp true nil
+   (TBind (TMem TBool TBool))
+   (TBind (TMem (TSelB 0) (TSelB 0))) n. (* can't do much with this *)
+Proof.
+  eexists. eapply stp_bindx.
+  instantiate (3 := (TMem TBool TBool)).
+  instantiate (2 := (TMem (TSel 0) (TSel 0))).
+
+  eapply stp_wrapf.
+  eapply stp_mem. eapply stp_wrapf.
+  eapply stp_sel1. compute. eauto. eapply stp_wrapf. eapply stp_mem. eauto. eauto. eauto. eauto.
+  eapply stp_sel2. compute. eauto. eauto.
+  eauto. eauto. 
+Grab Existential Variables. apply 0. apply 0. apply 0. apply 0. apply 0. apply 0. apply 0. 
+Qed.
+
 
 
 (* ############################################################ *)
@@ -276,8 +678,23 @@ Hint Constructors stp.
 
 
 Definition stpd b G1 T1 T2 := exists n, stp b G1 T1 T2 n.
+Definition itpd G1 T1 := exists n, itp G1 T1 n.
+
+Definition stpd2 b G1 T1 T2 := exists n, stp2 b G1 T1 T2 n.
+Definition itpd2 G1 T1 := exists n, itp2 G1 T1 n.
+
+Definition stpd3 b G1 T1 T2 := exists n, stp3 b G1 T1 T2 n.
+Definition itpd3 G1 T1 := exists n, itp3 G1 T1 n.
+
 
 Hint Unfold stpd.
+Hint Unfold itpd.
+
+Hint Unfold stpd2.
+Hint Unfold itpd2.
+
+Hint Unfold stpd3.
+Hint Unfold itpd3.
 
 Ltac ep := match goal with
              | [ |- stp ?M ?G1 ?T1 ?T2 ?N ] => assert (exists (x:nat), stp M G1 T1 T2 x) as EEX
@@ -285,8 +702,177 @@ Ltac ep := match goal with
 
 Ltac eu := match goal with
              | H: stpd _ _ _ _ |- _ => destruct H
-             | H: exists n: nat ,  _ |- _  => destruct H
+             | H: itpd _ _ |- _ => destruct H
+             | H: stpd2 _ _ _ _ |- _ => destruct H
+             | H: itpd2 _ _ |- _ => destruct H
+             | H: stpd3 _ _ _ _ |- _ => destruct H
+             | H: itpd3 _ _ |- _ => destruct H
+(*             | H: exists n: nat ,  _ |- _  =>
+               destruct H as [e P] *)
            end.
+
+Lemma stpd_bot: forall G1 T,
+    stpd true G1 TBot T.
+Proof. intros. exists 0. eauto. Qed.
+Lemma stpd_top: forall G1 T,
+    stpd true G1 T TTop.
+Proof. intros. exists 0. eauto. Qed.
+Lemma stpd_bool: forall G1,
+    stpd true G1 TBool TBool.
+Proof. intros. exists 0. eauto. Qed.
+Lemma stpd_fun: forall m G1 T11 T12 T21 T22,
+    stpd false G1 T21 T11 ->
+    stpd true G1 T12 T22 ->
+    stpd true G1 (TFun m T11 T12) (TFun m T21 T22).
+Proof. intros. repeat eu. eauto. Qed.
+Lemma stpd_mem: forall G1 T11 T12 T21 T22,
+    stpd false G1 T21 T11 ->
+    stpd true G1 T11 T12 ->
+    stpd true G1 T12 T22 ->
+    stpd true G1 (TMem T11 T12) (TMem T21 T22).
+Proof. intros. repeat eu. eauto. Qed.
+Lemma stpd_sel2: forall x T1 TX G1,
+    index x G1 = Some TX ->
+    stpd false G1 TX (TMem T1 TTop) ->
+    stpd true G1 T1 (TSel x).
+Proof. intros. repeat eu. eauto. Qed.
+Lemma stpd_sel1:  forall x T2 TX G1,
+    index x G1 = Some TX ->
+    stpd false G1 TX (TMem TBot T2) ->
+    stpd true G1 (TSel x) T2.
+Proof. intros. repeat eu. eauto. Qed.
+Lemma stpd_selx: forall x G1,
+    stpd true G1 (TSel x) (TSel x).
+Proof. intros. repeat eu. exists 1. eauto. Qed.
+Lemma stpd_bindx: forall G1 T1 T2 TA1 TA2,
+    stpd false ((length G1,T1)::G1) T1 T2 ->
+    open (length G1) TA1 = T1 ->                
+    open (length G1) TA2 = T2 ->
+    (* exp G1 T1 (TMem TL TU) -> *)
+    (* stpd true G1 TL TU -> *)
+    stpd true G1 (TBind TA1) (TBind TA2).
+Proof. intros. repeat eu. eauto. Qed.
+Lemma stpd_transf: forall G1 T1 T2 T3,
+    stpd true G1 T1 T2 ->
+    stpd false G1 T2 T3 ->           
+    stpd false G1 T1 T3.
+Proof. intros. repeat eu. eauto. Qed.
+Lemma stpd_wrapf: forall G1 T1 T2,
+    stpd true G1 T1 T2 ->
+    stpd false G1 T1 T2. 
+Proof. intros. repeat eu. eauto. Qed.
+
+Lemma stpd2_bot: forall G1 T,
+    stpd2 true G1 TBot T.
+Proof. intros. exists 0. eauto. Qed.
+Lemma stpd2_top: forall G1 T,
+    stpd2 true G1 T TTop.
+Proof. intros. exists 0. eauto. Qed.
+Lemma stpd2_bool: forall G1,
+    stpd2 true G1 TBool TBool.
+Proof. intros. exists 0. eauto. Qed.
+Lemma stpd2_fun: forall m G1 T11 T12 T21 T22,
+    stpd2 false G1 T21 T11 ->
+    stpd2 true G1 T12 T22 ->
+    stpd2 true G1 (TFun m T11 T12) (TFun m T21 T22).
+Proof. intros. repeat eu. eauto. Qed.
+Lemma stpd2_mem: forall G1 T11 T12 T21 T22,
+    stpd2 false G1 T21 T11 ->
+    stpd2 true G1 T11 T12 ->
+    stpd2 true G1 T12 T22 ->
+    stpd2 true G1 (TMem T11 T12) (TMem T21 T22).
+Proof. intros. repeat eu. eauto. Qed.
+Lemma stpd2_sel2: forall x T1 TX G1,
+    index x G1 = Some TX ->
+    itpd2 G1 TX ->
+    stpd2 true G1 TX (TMem T1 TTop) ->
+    stpd2 true G1 T1 (TSel x).
+Proof. intros. repeat eu. eauto. Qed.
+Lemma stpd2_sel1:  forall x T2 TX G1,
+    index x G1 = Some TX ->
+    itpd2 G1 TX ->
+    stpd2 true G1 TX (TMem TBot T2) ->
+    stpd2 true G1 (TSel x) T2.
+Proof. intros. repeat eu. eauto. Qed.
+Lemma stpd2_selx: forall x G1,
+    stpd2 true G1 (TSel x) (TSel x).
+Proof. intros. repeat eu. exists 1. eauto. Qed.
+Lemma stpd2_bindx: forall G1 T1 T2 TA1 TA2,
+    stpd false ((length G1,T1)::G1) T1 T2 -> (* !!! *)
+    open (length G1) TA1 = T1 ->                
+    open (length G1) TA2 = T2 ->
+    (* exp G1 T1 (TMem TL TU) -> *)
+    (* stpd true G1 TL TU -> *)
+    (* itpd2 ((length G1,T1)::G1) T1 -> *)
+    stpd2 true G1 (TBind TA1) (TBind TA2).
+Proof. intros. repeat eu. eauto. Qed.
+Lemma stpd2_transf: forall G1 T1 T2 T3,
+    stpd2 true G1 T1 T2 ->
+    stpd2 false G1 T2 T3 ->           
+    stpd2 false G1 T1 T3.
+Proof. intros. repeat eu. eauto. Qed.
+Lemma stpd2_wrapf: forall G1 T1 T2,
+    stpd2 true G1 T1 T2 ->
+    stpd2 false G1 T1 T2. 
+Proof. intros. repeat eu. eauto. Qed.
+
+
+Lemma stpd3_bot: forall G1 T,
+    stpd3 true G1 TBot T.
+Proof. intros. exists 0. eauto. Qed.
+Lemma stpd3_top: forall G1 T,
+    stpd3 true G1 T TTop.
+Proof. intros. exists 0. eauto. Qed.
+Lemma stpd3_bool: forall G1,
+    stpd3 true G1 TBool TBool.
+Proof. intros. exists 0. eauto. Qed.
+Lemma stpd3_fun: forall m G1 T11 T12 T21 T22,
+    stpd2 false G1 T21 T11 ->
+    stpd2 true G1 T12 T22 ->
+    stpd3 true G1 (TFun m T11 T12) (TFun m T21 T22).
+Proof. intros. repeat eu. info_eauto. Qed.
+Lemma stpd3_mem: forall G1 T11 T12 T21 T22,
+    stpd2 false G1 T21 T11 ->
+    stpd3 true G1 T12 T22 ->
+    stpd3 true G1 (TMem T11 T12) (TMem T21 T22).
+Proof. intros. repeat eu. eauto. Qed.
+Lemma stpd3_sel2: forall x T1 TX G1,
+    index x G1 = Some TX ->
+    itpd3 G1 TX ->
+    stpd3 true G1 TX (TMem T1 TTop) ->
+    stpd3 true G1 T1 (TSel x).
+Proof. intros. repeat eu. eauto. Qed.
+Lemma stpd3_sel1:  forall x T2 TX G1,
+    index x G1 = Some TX ->
+    itpd3 G1 TX ->
+    stpd3 true G1 TX (TMem TBot T2) ->
+    stpd3 true G1 (TSel x) T2.
+Proof. intros. repeat eu. eauto. Qed.
+Lemma stpd3_selx: forall x G1,
+    stpd3 true G1 (TSel x) (TSel x).
+Proof. intros. repeat eu. exists 1. eauto. Qed.
+Lemma stpd3_bindx: forall G1 T1 T2 TA1 TA2,
+    stpd3 true ((length G1,T1)::G1) T1 T2 -> (* !!! *)
+    open (length G1) TA1 = T1 ->                
+    open (length G1) TA2 = T2 ->
+    (* exp G1 T1 (TMem TL TU) -> *)
+    (* stpd true G1 TL TU -> *)
+    itpd3 ((length G1,T1)::G1) T1 -> 
+    stpd3 true G1 (TBind TA1) (TBind TA2).
+Proof. intros. repeat eu. eauto. Qed.
+Lemma stpd3_transf: forall G1 T1 T2 T3,
+    stpd3 true G1 T1 T2 ->
+    stpd3 false G1 T2 T3 ->           
+    stpd3 false G1 T1 T3.
+Proof. intros. repeat eu. eauto. Qed.
+Lemma stpd3_wrapf: forall G1 T1 T2,
+    stpd3 true G1 T1 T2 ->
+    stpd3 false G1 T1 T2. 
+Proof. intros. repeat eu. eauto. Qed.
+
+
+
+
 
 
 
@@ -295,6 +881,64 @@ Ltac index_subst := match goal with
                  | _ => idtac
                end.
 
+Lemma stp0f_trans: forall n n1 G1 T1 T2 T3,
+    stp false G1 T1 T2 n1 ->
+    stpd false G1 T2 T3 ->
+    n1 <= n ->
+    stpd false G1 T1 T3.
+Proof.
+  intros n. induction n.
+  - Case "z".
+    intros. assert (n1 = 0). omega. subst. inversion H.
+  - Case "S n".
+    intros. inversion H.
+    + eapply stpd_transf. eexists. eapply H2. eapply IHn. eapply H3. eapply H0. omega.
+    + destruct H0. eapply stpd_transf. eexists. eapply H2. eexists. eapply H0.
+Qed.  
+
+Lemma stp0f2_trans: forall n n1 G1 T1 T2 T3,
+    stp2 false G1 T1 T2 n1 ->
+    stpd2 false G1 T2 T3 ->
+    n1 <= n ->
+    stpd2 false G1 T1 T3.
+Proof.
+  intros n. induction n.
+  - Case "z".
+    intros. assert (n1 = 0). omega. subst. inversion H.
+  - Case "S n".
+    intros. inversion H.
+    + eapply stpd2_transf. eexists. eapply H2. eapply IHn. eapply H3. eapply H0. omega.
+    + destruct H0. eapply stpd2_transf. eexists. eapply H2. eexists. eapply H0.
+Qed.  
+
+
+
+(* implementable context *)
+Definition env_itp G := forall x T, index x G = Some T -> itpd G T.
+
+
+(* left:  may use axiom but has size. must shrink *)
+(* right: no axiom but can grow *)
+
+Definition trans_on n2 :=
+  forall m G1 T1 T2 T3,
+      stp2 m G1 T1 T2 n2 ->
+      stpd2 true G1 T2 T3 ->
+      stpd2 true G1 T1 T3.
+
+Hint Unfold trans_on.
+
+
+Definition trans_up n := forall n1, n1 <= n ->
+                      trans_on n1.
+Hint Unfold trans_up.
+
+Lemma trans_le: forall n n1,
+                      trans_up n ->
+                      n1 <= n ->
+                      trans_on n1
+.
+Proof. intros. unfold trans_up in H. eapply H. eauto. Qed.
 
 Lemma upd_length_same: forall {X} G x (T:X),
               length G = length (update x T G).
@@ -442,146 +1086,89 @@ Lemma stp_extend : forall m G1 T1 T2 x v n,
 Proof. admit. (*intros. destruct H. eexists. eapply stp_extend1. apply H.*) Qed.
 
 
-
-
-
-Fixpoint zeros d :=
-  match d with
-    | 0 => nil
-    | S n => 0::(zeros n)
-  end.
-
-
-Ltac mzero := match goal with
-             | H: _ :: _ = zeros ?d |- _ => destruct d; inversion H; simpl in H; inversion H
-           end.
-
-
-Lemma stp_trans0: forall n, forall n1 G1 T1 T2 T3 n2,
-      stp 0 G1 T1 T2 n1 -> n1 < n ->
-      stp 0 G1 T2 T3 n2 -> 
-      exists n3, stp 0 G1 T1 T3 n3. (* d2 <= d1 ? *)
+Lemma itp_extend: forall G T n x v,
+                         itp G T n ->
+                         itp ((x,v)::G) T n.
 Proof.
-  intros n. induction n; intros; inversion H; subst.
-  inversion H0. inversion H0. inversion H0. inversion H0.
-  - admit.
-  - admit.
-  - Case "wrapf". eexists. eapply stp_transf. eauto. eauto.
-  - Case "transf". admit.
+  admit. (* intros. induction H; eauto using index_extend. *)
 Qed.
 
 
-
-
-Lemma stp_trans1: forall n, forall n1 G1 T1 T2 T3 n2 d1 d2,
-      itp d2 T1 ->
-      stp d1 G1 T1 T2 n1 -> n1 < n ->
-      stp d2 G1 T2 T3 n2 -> d2 <= d1 ->
-      exists n3, stp d2 G1 T1 T3 n3. (* 0 < d1 ? *)
+(* currently n,n2 unrelated, but may change. keep in sync with env_itp definition *)
+Lemma env_itp_extend : forall G x v,  
+                       env_itp G ->
+                       itpd ((x,v)::G) v ->  
+                       env_itp ((x,v)::G).
 Proof.
-  intros n1. induction n1.
-  admit.
-  intros.
-  destruct d2.
-  (* zero: rhs may use trans *)
-  assert (stp 1 G1 T1 T2 n0). admit.  (* TODO: we have d1, but we need 1 !*)
-  eexists. eapply stp_transf. eauto. eauto.
-  (* > 0 no immediate trans in rhs *)
-  
-  inversion H0; subst.
-  - Case "bot". admit.
-  - Case "top". admit.
-  - Case "bool". admit.
-  - Case "fun". admit.
-  - Case "mem". inversion H2; subst.
-    + SCase "top". eauto.
-    + SCase "mem".
-      (* regular induction on upper bound *)
-      assert (exists n3, stp d2 G1 T12 T4 n3).
-      eapply IHn1. inversion H. eauto. eauto. omega. eauto. omega.
-      (* call zero case on lower bound (can't induct because taking from right) *)
-      assert (exists n3, stp 0 G1 T2 T11 n3).
-      eapply stp_trans0. eauto. eauto. eauto.
-      eu. eu.
-      eexists. eapply stp_mem; eauto.
-    + SCase "sel2".
-      inversion H7. subst. inversion H8. subst.
-      (* already need to invert TX < (TMem (TMem T4)) *)
-      assert (exists n3, stp 0 G1 (TMem T11 T12) T n3).
-      eapply stp_trans0. eauto. eauto. eauto.
-      eu.
-      (* now main rule *)
-      eexists. eapply stp_sel2. eauto. eauto. eapply stp_mem; eauto.
-  - Case "sel2". inversion H1; subst.
-    + SCase "top". admit.
-    + SCase "sel2". admit.
-    + SCase "sel1". admit. (**)
-    + SCase "selx". admit.
-    + SCase "wrap". admit.
-    + SCase "trans". admit.
-  - Case "sel1". admit.
-  - Case "selx". admit.
-  - Case "bindx". admit. (**)
-  - Case "wrapf". admit. (**)
-  - Case "trans". admit.
+  intros. unfold env_itp in H. unfold env_itp. intros.
+  case_eq (beq_nat x0 (length G)); intros.
+  - assert (x0 = (length G)). eapply beq_nat_true_iff; eauto.
+    subst x0. unfold index in H1. rewrite H2 in H1. inversion H1. subst v.
+    eapply H0.
+  - assert (x0 <> (length G)). eapply beq_nat_false_iff; eauto.
+    assert (x0 < length ((x,v)::G)). eapply index_max; eauto.
+    
+    unfold index in H1. rewrite H2 in H1.
+    eapply H in H1. destruct H1. eexists. eapply itp_extend. apply H1.
 Qed.
-
 
 Lemma stp_narrow: forall n, forall m G1 T1 T2 n1 n0,
-  stp m G1 T1 T2 n0 -> n0 < n ->                  
-  forall x TX1 TX2 G1' d2,
+  stp m G1 T1 T2 n0 ->
+  n0 <= n ->                    
+  forall x TX1 TX2 G1',
+
     index x G1 = Some TX2 ->
     update x TX1 G1 = G1' ->
-    stp d2 G1' TX1 TX2 n1 -> m <= d2 ->
-    exists n3, stp m G1' T1 T2 n3.
+    stp false G1' TX1 TX2 n1 ->
+    stpd m G1' T1 T2.
 Proof.
-  intros n. induction n.
-  (* z *) intros. admit. 
+  intros n.
+  induction n.
+  (* z *) intros. inversion H0. subst. inversion H; eauto.
   (* s n *)
-  intros m G1 T1 T2 n1 nz H NE.
+  intros m G1 T1 T2 n1 n0 H NE.
   inversion H; intros.
-  - Case "Top". admit. 
-  - Case "Bool". admit. 
-  - Case "Fun". admit.
-  - Case "Mem". subst.
-    assert (exists n3 : nat, stp 0 (update x TX1 G1) T3 T0 n3).
-    eapply IHn; eauto. omega. omega.
-    assert (exists n3 : nat, stp d2 (update x TX1 G1) T0 T3 n3).
-    eapply IHn; eauto. omega. omega.
-    eu. eu.
-    eexists. eapply stp_mem; eauto.
+  - Case "Bot".
+    intros. eapply stpd_bot.
+  - Case "Top".
+    intros. eapply stpd_top.
+  - Case "Bool". 
+    intros. eapply stpd_bool.
+  - Case "Fun". 
+    intros. eapply stpd_fun. eapply IHn; eauto. omega. eapply IHn; eauto. omega.
+  - Case "Mem". 
+    intros. eapply stpd_mem. eapply IHn; eauto. omega. eapply IHn; eauto. omega. eapply IHn; eauto. omega.
   - Case "Sel2". intros.
     { case_eq (beq_nat x x0); intros E.
       (* hit updated binding *)
       + assert (x = x0) as EX. eapply beq_nat_true_iff; eauto. subst. index_subst. index_subst.
-
-        (* narrow ind *)
-        assert (exists n3, stp m (update x0 TX1 G1) TX (TMem T1) n3).
-        eapply IHn. eauto. omega. eauto. eauto. eauto. omega.
-        eu.
-        
-        (* trans with delta *)
-        assert (exists n3, stp m (update x0 TX1 G1) TX1 (TMem T1) n3).
-        eapply stp_trans1. eauto. eauto. eauto. omega.
-        eu.
-        
-        eexists. eapply stp_sel2. eapply upd_hit; eauto. eauto.
-
+        eapply stpd_sel2. eapply upd_hit; eauto.
+        (* trans, and narrow by induction *)
+        eapply stp0f_trans. eapply H9. eapply IHn; eauto. omega. eauto.
+      (* other binding *)
       + assert (x <> x0) as EX. eapply beq_nat_false_iff; eauto.
-        assert (exists n3, stp m G1' TX (TMem T1) n3).
+        eapply stpd_sel2. eapply upd_miss; eauto.
+        (* narrow stp by induction *)
         eapply IHn; eauto. omega.
-        eu.
-
-        eexists. eapply stp_sel2. eapply upd_miss; eauto. eauto.
     }
-  - Case "Sel1". admit.
-  - Case "Selx". admit.
+  - Case "Sel1". intros.
+    { case_eq (beq_nat x x0); intros E.
+      (* hit updated binding *)
+      + assert (x = x0) as EX. eapply beq_nat_true_iff; eauto. subst. index_subst. index_subst. 
+        eapply stpd_sel1. eapply upd_hit; eauto.
+        (* trans, and narrow by induction *)
+        eapply stp0f_trans. eapply H9. eapply IHn; eauto. omega. eauto.
+      (* other binding *)
+      + assert (x <> x0) as EX. eapply beq_nat_false_iff; eauto.
+        eapply stpd_sel1. eapply upd_miss; eauto.
+        (* narrow stp by induction *)
+        eapply IHn; eauto. omega.
+    }
+  - Case "Selx". eapply stpd_selx.
   - Case "Bindx".
     assert (length G1 = length G1'). { eapply update_pres_len; eauto. }
     remember (length G1) as L. clear HeqL. subst L.
 
-    admit.
-    (*
     eapply stpd_bindx. {
       eapply IHn. eapply H0. omega.
       eapply index_extend; eauto.
@@ -589,11 +1176,12 @@ Proof.
       eapply stp_extend; eauto.
     }
     eauto.
-    eauto. *)
+    eauto.
 
-  - Case "Wrap". admit. (* eapply stpd_wrapf. eapply IHn; eauto. omega. *)
-  - Case "Trans". admit. (*eapply stpd_transf. eapply IHn; eauto. omega. eapply IHn; eauto. omega. *)
+  - Case "Trans". eapply stpd_transf. eapply IHn; eauto. omega. eapply IHn; eauto. omega.
+  - Case "Wrap". eapply stpd_wrapf. eapply IHn; eauto. omega.
 
+    Grab Existential Variables. apply 0. apply 0. apply 0.
 Qed.
 
 
@@ -920,8 +1508,9 @@ Proof.
   - Case "mem".
     inversion H0. subst.
     assert (trans_on n5) as IH. { eapply trans_le; eauto. omega. }
-
     eapply stpd2_mem. eauto. eauto. eapply IH. eauto. eauto.
+  - Case "bind".
+    inversion H3.
   - Case "sel".
     inversion H3. subst. index_subst.
     assert (trans_up n2) as IH. { unfold trans_up. intros. eapply trans_le; eauto. omega. }
@@ -966,6 +1555,8 @@ Proof.
     + SCase "trivial nest".
       inversion H0. inversion H1. subst. inversion H3. subst.
       eapply stpd2_mem. eauto. eauto. eapply IHitp. eauto. eauto. eauto.
+  - Case "bind".
+    inversion H0; subst; inversion H3.
   - Case "sel".
     inversion H0.
     + SCase "trivial mem". subst.
@@ -1179,6 +1770,98 @@ Proof.
       eapply stpd2_wrapf. eapply IHn; eauto. omega.
 Grab Existential Variables. apply 0. apply 0. apply 0. apply 0. apply 0. apply 0. apply 0.
 Qed.
+
+(* ----------- stp3 code --------- *)
+
+
+Definition trans_on3 n2 :=
+  forall m G1 T1 T2 T3,
+      stp3 m G1 T1 T2 n2 ->
+      stpd3 true G1 T2 T3 ->
+      stpd3 true G1 T1 T3.
+
+Hint Unfold trans_on3.
+
+
+Definition trans_up3 n := forall n1, n1 <= n ->
+                      trans_on3 n1.
+Hint Unfold trans_up3.
+
+(* proper trans lemma *)
+Lemma stp3_trans: forall n, trans_up3 n.
+Proof.
+admit. Qed.
+
+
+Lemma stp3_untrans: forall n, forall G1 T1 T2 n0,
+  stp3 false G1 T1 T2 n0 ->
+  n0 <= n ->
+  stpd3 true G1 T1 T2.
+Proof.
+  intros n. induction n.
+  - Case "z".
+    intros. inversion H; inversion H0; subst; eauto; try solve by inversion.
+  - Case "s n".
+    intros. inversion H; subst.
+    + SCase "transf". eapply stp3_trans.
+      instantiate (2 := n1).
+      instantiate (1 := n1).
+      eauto. eapply H1. eapply IHn. eauto. omega. 
+    + SCase "wrapf". eauto.
+Qed.
+
+Lemma itp_widen: forall G1 T1 T2 n1,
+  itp3 G1 T1 n1 ->
+  stpd3 true G1 T1 T2 ->
+  itpd3 G1 T2.
+Proof. admit. Qed.
+
+Lemma stp_convert3: forall n, forall m G1 T1 T2 n0 n1,
+  itp3 G1 T1 n1 ->
+  stp m G1 T1 T2 n0 ->
+  n0 <= n ->
+  env_itp G1 ->
+  stpd3 true G1 T1 T2.
+Proof.
+  intros n.
+  induction n.
+  - Case "z".
+    intros. inversion H0; inversion H1; subst; eauto; try solve by inversion.
+  - Case "s n".
+    intros.
+    inversion H0.
+    + SCase "bot". eauto.
+    + SCase "top". eauto.
+    + SCase "bool". eauto.
+    + SCase "fun". eapply stpd3_fun. eapply stp_convert; eauto. eapply stp_convert; eauto.
+    + SCase "mem". eapply stpd3_mem. eapply stp_convert; eauto. subst. inversion H. subst. eapply IHn; eauto. omega. 
+    + SCase "sel2".
+      assert (itpd3 G1 TX). { eapply H2; eauto. } (* from env_itp *)
+      assert (stpd3 true G1 TX (TMem T1 TTop)) as ST. { eu. eapply IHn; eauto. omega. }
+      eapply stpd3_sel2; eauto.
+    + SCase "sel1".
+      assert (itpd3 G1 TX). { eapply H2; eauto. } (* from env_itp *)
+      assert (stpd3 true G1 TX (TMem TBot T2)) as ST. { eu. eapply IHn; eauto. omega. }
+      eapply stpd3_sel1; eauto.
+    + SCase "selx".
+      eapply stpd3_selx; eauto.
+    + SCase "bindx".
+      eapply stpd3_bindx. subst. inversion H. subst.
+      eapply IHn. eauto. eauto. omega. eapply env_itp_extend; eauto. subst. eauto. subst. eauto.
+      subst. inversion H. subst. eauto.
+    + SCase "transf".
+      assert (itpd3 G1 T3). { eapply itp_widen; eauto.  eapply IHn; eauto. omega. } eu.
+      assert (stpd3 false G1 T1 T2). eapply stpd3_transf. eapply IHn; eauto. omega. eapply stpd3_wrapf. eapply IHn; eauto. omega. eu.
+      eapply stp3_untrans; eauto.
+    + SCase "wrapf".
+      eapply IHn; eauto. omega.
+Grab Existential Variables. apply 0. apply 0. apply 0. apply 0. apply 0. apply 0. apply 0.
+Qed.
+
+
+
+
+
 
 End DOT.
 
